<!-- 证明：若d(n)为O(f(n))，e(n)为O(g(n)，则d(n)+e(n)为O(f(n)+g(n))。 -->

### 证明：若 \(d(n) = O(f(n))\) 且 \(e(n) = O(g(n))\)，则 \(d(n) + e(n) = O(f(n) + g(n))\)

#### 证明过程如下：

1. **根据大O记号定义：**  
   由 \(d(n) = O(f(n))\)，存在常数 \(c_1 > 0\) 和 \(n_1 > 0\)，使得对所有 \(n \geq n_1\)：  
   \[ 0 \leq d(n) \leq c_1 \cdot f(n) \]

   由 \(e(n) = O(g(n))\)，存在常数 \(c_2 > 0\) 和 \(n_2 > 0\)，使得对所有 \(n \geq n_2\)：  
   \[ 0 \leq e(n) \leq c_2 \cdot g(n) \]

2. **构造新常数：**  
   定义：  
   \[ c = c_1 + c_2 \]  
   \[ n_0 = \max(n_1, n_2) \]

3. **分析相加函数：**  
   当 \(n \geq n_0\) 时（即同时满足 \(n \geq n_1\) 且 \(n \geq n_2\)）：  
   \[ \begin{align*}
   d(n) + e(n) &\leq c_1 \cdot f(n) + c_2 \cdot g(n) \\
   &\leq c_1 \cdot f(n) + c_2 \cdot g(n) + c_1 \cdot g(n) + c_2 \cdot f(n) \\
   &= (c_1 + c_2) \cdot f(n) + (c_1 + c_2) \cdot g(n) \\
   &= c \cdot (f(n) + g(n))
   \end{align*} \]

4. **验证大O定义：**  
   对所有 \(n \geq n_0\)，有：  
   \[ 0 \leq d(n) + e(n) \leq c \cdot (f(n) + g(n)) \]  
   满足 \(O(f(n) + g(n))\) 的定义条件。

---

#### 结论：

存在常数 \(c = c_1 + c_2 > 0\) 和 \(n_0 = \max(n_1, n_2) > 0\)，  
使得对所有 \(n \geq n_0\)，不等式 \(d(n) + e(n) \leq c \cdot (f(n) + g(n))\) 成立。  
因此：  
\[ \boxed{d(n) + e(n) = O(f(n) + g(n))} \]
