<!-- 证明：O(max{f(n),g(n)})=O(f(n)+g(n))。 -->

### 证明：\( O(\max\{f(n), g(n)\}) = O(f(n) + g(n)) \)

#### 证明思路：

1. 证明 \( O(\max\{f(n), g(n)\}) \subseteq O(f(n) + g(n)) \)
2. 证明 \( O(f(n) + g(n)) \subseteq O(\max\{f(n), g(n)\}) \)

假设 \( f(n), g(n) \geq 0 \)（标准假设）。

---

#### 第 1 部分：\( O(\max\{f,g\}) \subseteq O(f+g) \)

设 \( h(n) \in O(\max\{f(n), g(n)\}) \)，则存在 \( c_1 > 0 \), \( n_1 > 0 \) 使得：  
\[ \forall n \geq n_1,\ \ 0 \leq h(n) \leq c_1 \cdot \max\{f(n), g(n)\} \]  
由 \( \max\{f,g\} \leq f + g \)：  
\[ h(n) \leq c_1 \cdot (f(n) + g(n)) \]  
故 \( h(n) \in O(f(n) + g(n)) \).

#### 第 2 部分：\( O(f+g) \subseteq O(\max\{f,g\}) \)

设 \( h(n) \in O(f(n) + g(n)) \)，则存在 \( c_2 > 0 \), \( n_2 > 0 \) 使得：  
\[ \forall n \geq n_2,\ \ 0 \leq h(n) \leq c_2 \cdot (f(n) + g(n)) \]  
由 \( f + g \leq 2 \cdot \max\{f,g\} \)：  
\[ h(n) \leq 2c_2 \cdot \max\{f(n), g(n)\} \]  
故 \( h(n) \in O(\max\{f(n), g(n)\}) \).

---

#### 结论：

\[
\boxed{O(\max\{f(n), g(n)\}) = O(f(n) + g(n))}
\]
